1. Progress in DIjkstra; pausing until OOPSLA camera-ready 2. Polishing throughout paper 3. Additions to related work: resolves issue 34

sample_mark/verif_dijkstra.v
@@ -21,4 +21,38 @@ Definition whole_graph sh g x := (@graph_rep_spatial mpred pointer_val (SDAG_VST
 (* 				mypath = path *)
 
 
-                                           
+Definition dijkstra_correct (g: Graph) p src dst : Prop :=
+    path_ends g p src dst ->
+    forall p', path_ends g p' src dst ->
+               Nat.lt (path_cost g p') (path_cost g p) ->
+               p = p'.
+         
+Definition dijkstra_spec :=
+  DECLARE _dijkstra
+  WITH sh: wshare, g: Graph, arr: pointer_val,
+       dist: pointer_val, prev: pointer_val,
+       i: Z, src: Z, dst: Z
+  PRE []
+    PROP ()
+    LOCAL () (* temp _pq (pointer_val_val arr); temp _i (Vint (Int.repr i))) *)
+    SEP (whole_graph sh g arr)
+  POST [tvoid]
+      EX p : (@path VType EType),
+      PROP (dijkstra_correct g p src dst)
+      LOCAL ()
+      SEP (whole_graph sh g arr).
+
+Definition Gprog : funspecs := ltac:(with_library prog [dijkstra_spec]).
+
+Lemma body_find: semax_body Vprog Gprog f_dijkstra dijkstra_spec.
+Proof.
+  start_function.
+  forward.
+  forward_for_simple_bound 8 
+    (EX i: Z,
+    PROP  ()
+    LOCAL (lvar _pq (tptr (Tstruct _Node noattr)) v_pq)
+    SEP (data_at Tsh (tptr (Tstruct _Node noattr)) (Vint (Int.repr 0)) v_pq;
+         whole_graph sh g arr)).
+  - entailer!.
+    Abort.
